Uppaal_Networks/AbsInt/Word.thy
@@ -11,9 +11,21 @@ locale AbsWord =
 fixes \<gamma>_word :: "('a::absword) \<Rightarrow> int set"
   and aplus :: "'a \<Rightarrow> 'a \<Rightarrow> 'a"
   and contains :: "'a \<Rightarrow> int \<Rightarrow> bool"
+  and lt :: "'a \<Rightarrow> 'a \<Rightarrow> power_bool"
+  and le :: "'a \<Rightarrow> 'a \<Rightarrow> power_bool"
+  and eq :: "'a \<Rightarrow> 'a \<Rightarrow> power_bool"
 assumes mono_gamma: "a \<le> b \<Longrightarrow> \<gamma>_word a \<le> \<gamma>_word b"
-  and gamma_Top[simp]: "\<gamma>_word \<top> = UNIV"
+  and gamma_Top[simp]: "\<gamma>_word \<top> = \<top>"
   and plus_correct: "x \<in> \<gamma>_word a \<Longrightarrow> y \<in> \<gamma>_word b \<Longrightarrow> (x + y) \<in> \<gamma>_word (aplus a b)"
   and contains_correct: "contains a x \<longleftrightarrow> x \<in> \<gamma>_word a"
+  and lt_correct: "lt a b = (     if \<forall>x y. x \<in> \<gamma>_word a \<longrightarrow> y \<in> \<gamma>_word b \<longrightarrow> x < y then BTrue
+                             else if \<exists>x y. x \<in> \<gamma>_word a \<longrightarrow> y \<in> \<gamma>_word b \<longrightarrow> x < y then BBoth
+                             else BFalse)"
+  and le_correct: "le a b = (     if \<forall>x y. x \<in> \<gamma>_word a \<longrightarrow> y \<in> \<gamma>_word b \<longrightarrow> x \<le> y then BTrue
+                             else if \<exists>x y. x \<in> \<gamma>_word a \<longrightarrow> y \<in> \<gamma>_word b \<longrightarrow> x \<le> y then BBoth
+                             else BFalse)"
+  and eq_correct: "eq a b = (     if \<forall>x y. x \<in> \<gamma>_word a \<longrightarrow> y \<in> \<gamma>_word b \<longrightarrow> x = y then BTrue
+                             else if \<exists>x y. x \<in> \<gamma>_word a \<longrightarrow> y \<in> \<gamma>_word b \<longrightarrow> x = y then BBoth
+                             else BFalse)"
 
 end
